par permute lemmas

Pom/Lpo/Operations/Par/Isomorphism.lean
@@ -4,13 +4,31 @@ import Pom.Lpo.Operations.Seq.Equiv
 
 namespace Lpo
 
-noncomputable def Equiv.par {x y : Node} {X X' Y Y' : Set Node} (e₁ : X ≃ Y) (e₂ : X' ≃ Y')
+namespace Equiv
+
+noncomputable def par {x y : Node} {X X' Y Y' : Set Node} (e₁ : X ≃ Y) (e₂ : X' ≃ Y')
     (hx : x ∉ X) (hx' : x ∉ X') (hd : Disjoint X X')
     (hy : y ∉ Y) (hy' : y ∉ Y') (hd' : Disjoint Y Y') :
     ↑(Set.insert x (X ∪ X')) ≃ ↑(Set.insert y (Y ∪ Y')) :=
   (Equiv.singleton x y).union (e₁.union e₂ hd hd')
     (by refine Set.disjoint_left.mpr ?_; rintro x rfl (h | h) <;> contradiction)
     (by refine Set.disjoint_left.mpr ?_; rintro x rfl (h | h) <;> contradiction)
+
+lemma root_eq_par_symm {x y : Node} {X X' Y Y' : Set Node} {e₁ : X ≃ Y} {e₂ : X' ≃ Y'}
+    {hx : x ∉ X} {hx' : x ∉ X'} {hd : Disjoint X X'}
+    {hy : y ∉ Y} {hy' : y ∉ Y'} {hd' : Disjoint Y Y'}
+    {z : Node} {hz : z ∈ Set.insert y (Y ∪ Y')}
+    (heq : x = ((Equiv.par e₁ e₂ hx hx' hd hy hy' hd').symm ⟨z, hz⟩)) :
+    y = z := by
+  suffices h : Subtype.mk y (Set.mem_insert _ _) = ⟨z, hz⟩ from congrArg Subtype.val h
+  refine (Equiv.par e₁ e₂ hx hx' hd hy hy' hd').symm.injective ?_
+  ext; refine Eq.trans ?_ heq
+  conv => lhs; exact Equiv.union_symm_apply_left (Set.mem_singleton _)
+  rfl
+
+end Equiv
+
+section ParPermute
 
 lemma par_form₁ {φ : Form Node} {x y : Node} (hφ : Form.literal x ≤ φ ∧ φ.DependsOn {x}) :
     Form.literal y ≤ φ.permute (Equiv.singleton x y) ∧
@@ -50,7 +68,7 @@ lemma par_form₂ {φ : Form Node} {x y : Node} (hφ : (Form.literal x).not ≤ 
     obtain ⟨w, _, hmem⟩ := himg
     simpa only [Set.mem_singleton_iff.mp w.property] using hmem
 
-lemma par_permute {l : Type} [Bot l] {x : Node} {ℓ : l} {α β : Lpo l}
+variable {l : Type} [Bot l] {x : Node} {ℓ : l} {α β : Lpo l}
     {φ₁ φ₂ : Form Node}
     {hx : x ∉ α.nodes} {hx' : x ∉ β.nodes}
     {hd : Disjoint α.nodes β.nodes}
@@ -59,15 +77,231 @@ lemma par_permute {l : Type} [Bot l] {x : Node} {ℓ : l} {α β : Lpo l}
     {hφ₂ : (Form.literal x).not ≤ φ₂ ∧ φ₂.DependsOn {x}}
     {X Y : Set Node} {y : Node}
     (hy : y ∉ X) (hy' : y ∉ Y) (hd' : Disjoint X Y)
-    (e₁ : α.nodes ≃ X) (e₂ : β.nodes ≃ Y) :
+    (e₁ : α.nodes ≃ X) (e₂ : β.nodes ≃ Y)
+
+lemma par_permute_rel :
+    ((par_gen hx hx' hd hroot hφ₁ hφ₂).permute (Equiv.par e₁ e₂ hx hx' hd hy hy' hd')).rel =
+    (par_gen (α := α.permute e₁) (β := β.permute e₂)
+      hy hy' hd' hroot (par_form₁ hφ₁) (par_form₂ hφ₂)).rel := by
+  ext u v; constructor
+  · rintro ⟨hu, _, ⟨heq, hv⟩ | hrel | hrel⟩
+    · left; constructor
+      · exact Equiv.root_eq_par_symm heq
+      · exact Equiv.mem_union_symm_right hv
+    · right; left; have ⟨hu, hv⟩ := α.property.rel_dom hrel
+      have hu' : _ ∈ α.nodes ∪ β.nodes := Or.inl hu
+      have hv' : _ ∈ α.nodes ∪ β.nodes := Or.inl hv
+      conv at hu =>
+        rhs; exact Equiv.union_symm_apply_right <| Equiv.mem_union_symm_right hu'
+      conv at hv =>
+        rhs; exact Equiv.union_symm_apply_right <| Equiv.mem_union_symm_right hv'
+      conv at hrel =>
+        arg 2; exact Equiv.union_symm_apply_right <| Equiv.mem_union_symm_right hu'
+      conv at hrel =>
+        arg 3; exact Equiv.union_symm_apply_right <| Equiv.mem_union_symm_right hv'
+      have hu' := Equiv.mem_union_symm_left hu; have hv' := Equiv.mem_union_symm_left hv
+      conv at hrel => arg 2; exact Equiv.union_symm_apply_left hu'
+      conv at hrel => arg 3; exact Equiv.union_symm_apply_left hv'
+      exact ⟨hu', hv', hrel⟩
+    · right; right; have ⟨hu, hv⟩ := β.property.rel_dom hrel
+      have hu' : _ ∈ α.nodes ∪ β.nodes := Or.inr hu
+      have hv' : _ ∈ α.nodes ∪ β.nodes := Or.inr hv
+      conv at hu =>
+        rhs; exact Equiv.union_symm_apply_right <| Equiv.mem_union_symm_right hu'
+      conv at hv =>
+        rhs; exact Equiv.union_symm_apply_right <| Equiv.mem_union_symm_right hv'
+      conv at hrel =>
+        arg 2; exact Equiv.union_symm_apply_right <| Equiv.mem_union_symm_right hu'
+      conv at hrel =>
+        arg 3; exact Equiv.union_symm_apply_right <| Equiv.mem_union_symm_right hv'
+      have hu' := Equiv.mem_union_symm_right hu; have hv' := Equiv.mem_union_symm_right hv
+      conv at hrel => arg 2; exact Equiv.union_symm_apply_right hu'
+      conv at hrel => arg 3; exact Equiv.union_symm_apply_right hv'
+      exact ⟨hu', hv', hrel⟩
+  · rintro (⟨rfl, hv⟩ | ⟨hu, hv, hrel⟩ | ⟨hu, hv, hrel⟩)
+    · refine ⟨Set.mem_insert _ _, ?_, ?_⟩
+      · right; exact hv
+      · left; constructor
+        · conv => rhs; exact Equiv.union_symm_apply_left (Set.mem_singleton _)
+          rfl
+        · conv => rhs; exact Equiv.union_symm_apply_right hv
+          exact Subtype.coe_prop _
+    · refine ⟨Or.inr <| Or.inl hu, Or.inr <| Or.inl hv, ?_⟩
+      right; left
+      have hu' : u ∈ X ∪ Y := Or.inl hu
+      have hv' : v ∈ X ∪ Y := Or.inl hv
+      conv =>
+        arg 2; exact (Equiv.union_symm_apply_right hu').trans <| Equiv.union_symm_apply_left hu
+      conv =>
+        arg 3; exact (Equiv.union_symm_apply_right hv').trans <| Equiv.union_symm_apply_left hv
+      exact hrel
+    · refine ⟨Or.inr <| Or.inr hu, Or.inr <| Or.inr hv, ?_⟩
+      right; right
+      have hu' : u ∈ X ∪ Y := Or.inr hu
+      have hv' : v ∈ X ∪ Y := Or.inr hv
+      conv =>
+        arg 2; exact (Equiv.union_symm_apply_right hu').trans <| Equiv.union_symm_apply_right hu
+      conv =>
+        arg 3; exact (Equiv.union_symm_apply_right hv').trans <| Equiv.union_symm_apply_right hv
+      exact hrel
+
+lemma par_permute_lab :
+    ((par_gen hx hx' hd hroot hφ₁ hφ₂).permute (Equiv.par e₁ e₂ hx hx' hd hy hy' hd')).lab =
+    (par_gen (α := α.permute e₁) (β := β.permute e₂)
+      hy hy' hd' hroot (par_form₁ hφ₁) (par_form₂ hφ₂)).lab := by
+  ext z; by_cases hz : z ∈ Set.insert y (X ∪ Y)
+  · conv => lhs; exact dif_pos hz
+    classical
+    refine dite_congr ?_ (fun _ ↦ rfl) (fun hne ↦ ?_)
+    · ext; constructor
+      · exact Equiv.root_eq_par_symm
+      · rintro rfl
+        conv => rhs; exact Equiv.union_symm_apply_left (Set.mem_singleton _)
+        rfl
+    · have hz := Set.mem_of_mem_insert_of_ne hz (Ne.symm hne)
+      refine if_congr ?_ ?_ ?_
+      · conv => lhs; rhs; exact Equiv.union_symm_apply_right hz
+        constructor
+        · exact Equiv.mem_union_symm_left
+        · intro hz; conv => rhs; exact Equiv.union_symm_apply_left hz
+          exact Subtype.coe_prop _
+      · conv => lhs; arg 2; exact Equiv.union_symm_apply_right hz
+        rcases hz with hz | hz
+        · conv => lhs; arg 2; exact Equiv.union_symm_apply_left hz
+          symm; exact dif_pos hz
+        · conv => rhs; exact dif_neg (Set.disjoint_right.mp hd' hz)
+          refine α.property.lab_dom _ (Set.disjoint_right.mp hd ?_)
+          conv => rhs; exact Equiv.union_symm_apply_right hz
+          exact Subtype.coe_prop _
+      · conv => lhs; arg 2; exact Equiv.union_symm_apply_right hz
+        rcases hz with hz | hz
+        · conv => rhs; exact dif_neg (Set.disjoint_left.mp hd' hz)
+          refine β.property.lab_dom _ (Set.disjoint_left.mp hd ?_)
+          conv => rhs; exact Equiv.union_symm_apply_left hz
+          exact Subtype.coe_prop _
+        · conv => lhs; arg 2; exact Equiv.union_symm_apply_right hz
+          symm; exact dif_pos hz
+  · conv => lhs; exact dif_neg hz
+    symm; exact (par_gen _ _ _ _ _ _).property.lab_dom _ hz
+
+lemma and_congr_with_h {P P' Q Q' : Prop}
+    (h : P ↔ P') (h' : P → P' → (Q ↔ Q')) : P ∧ Q ↔ P' ∧ Q' := by
+  have := iff_iff_eq.mp h; subst this
+  exact and_congr_right (fun p ↦ h' p p)
+
+lemma par_permute_form :
+    ((par_gen hx hx' hd hroot hφ₁ hφ₂).permute (Equiv.par e₁ e₂ hx hx' hd hy hy' hd')).form =
+    (par_gen (α := α.permute e₁) (β := β.permute e₂)
+      hy hy' hd' hroot (par_form₁ hφ₁) (par_form₂ hφ₂)).form := by
+  ext z v; by_cases hz : z ∈ Set.insert y (X ∪ Y)
+  · refine (exists_prop_of_true hz).trans ?_
+    refine or_congr ?_ (or_congr ?_ ?_)
+    · constructor
+      · exact Equiv.root_eq_par_symm
+      · rintro rfl; conv => rhs; exact Equiv.union_symm_apply_left (Set.mem_singleton y)
+        rfl
+    · refine and_congr_with_h ?_ ?_
+      · constructor
+        · intro h; have := Equiv.mem_union_symm_right <| Set.mem_union_left _ h
+          conv at h => rhs; exact Equiv.union_symm_apply_right this
+          exact Equiv.mem_union_symm_left h
+        · intro h;
+          conv => rhs; exact Equiv.union_symm_apply_right (Set.mem_union_left _ h)
+          conv => rhs; exact Equiv.union_symm_apply_left h
+          exact Subtype.coe_prop _
+      · intro h h'; refine and_congr ?_ ?_
+        · refine Iff.trans ?_ (exists_prop_of_true h').symm
+          conv => lhs; arg 2; exact Equiv.union_symm_apply_right (Set.mem_union_left _ h')
+          conv => lhs; arg 2; exact Equiv.union_symm_apply_left h'
+          refine iff_iff_eq.mpr <| (α.property.form _ (Subtype.coe_prop _)).1 _ _ ?_
+          refine Set.disjoint_left.mpr ?_; intro w hsd hrel
+          have hw := (α.property.rel_dom hrel).1; clear hrel
+          rcases Set.mem_symmDiff.mp hsd with ⟨⟨⟨u, hu⟩, rfl, hv⟩, h'⟩ | ⟨⟨⟨u, hu⟩, rfl, hv⟩, h'⟩
+          · simp only [Form.image, Subtype.exists, exists_and_right, Set.mem_setOf_eq, not_exists,
+              not_and, forall_exists_index] at h'
+            have := Equiv.mem_union_symm_right <| Set.mem_union_left _ hw
+            conv at hw => rhs; exact Equiv.union_symm_apply_right this
+            have hu := Equiv.mem_union_symm_left hw
+            refine h' _ hu ?_ hv
+            symm; conv => lhs; exact Equiv.union_symm_apply_right this
+            exact Equiv.union_symm_apply_left hu
+          · simp only [Form.image, Subtype.exists, exists_and_right, Set.mem_setOf_eq, not_exists,
+              not_and, forall_exists_index] at h'
+            refine h' u (Or.inr (Or.inl hu)) ?_ hv
+            conv => lhs; exact Equiv.union_symm_apply_right <| Set.mem_union_left _ hu
+            exact Equiv.union_symm_apply_left hu
+        · refine iff_iff_eq.mpr <| hφ₁.2 _ _ ?_
+          refine Set.disjoint_left.mpr ?_; rintro x hsd rfl
+          rcases Set.mem_symmDiff.mp hsd with ⟨⟨⟨u, hu⟩, heq, hv⟩, h'⟩ | ⟨⟨⟨u, rfl⟩, heq, hv⟩, h'⟩
+          · simp only [Form.image, Subtype.exists, exists_and_right, Set.mem_setOf_eq, not_exists,
+              not_and, forall_exists_index] at h'
+            obtain rfl := Equiv.root_eq_par_symm heq.symm
+            exact h' _ (Set.mem_singleton _) rfl hv
+          · simp only [Form.image, Subtype.exists, exists_and_right, Set.mem_setOf_eq, not_exists,
+              not_and, forall_exists_index] at h'
+            refine h' _ (Set.mem_insert _ _) ?_ hv
+            conv => rhs; exact heq.symm
+            exact Equiv.union_symm_apply_left (Set.mem_singleton _)
+    · refine and_congr_with_h ?_ ?_
+      · constructor
+        · intro h; have := Equiv.mem_union_symm_right <| Set.mem_union_right _ h
+          conv at h => rhs; exact Equiv.union_symm_apply_right this
+          exact Equiv.mem_union_symm_right h
+        · intro h;
+          conv => rhs; exact Equiv.union_symm_apply_right (Set.mem_union_right _ h)
+          conv => rhs; exact Equiv.union_symm_apply_right h
+          exact Subtype.coe_prop _
+      · intro h h'; refine and_congr ?_ ?_
+        · refine Iff.trans ?_ (exists_prop_of_true h').symm
+          conv => lhs; arg 2; exact Equiv.union_symm_apply_right (Set.mem_union_right _ h')
+          conv => lhs; arg 2; exact Equiv.union_symm_apply_right h'
+          refine iff_iff_eq.mpr <| (β.property.form _ (Subtype.coe_prop _)).1 _ _ ?_
+          refine Set.disjoint_left.mpr ?_; intro w hsd hrel
+          have hw := (β.property.rel_dom hrel).1; clear hrel
+          rcases Set.mem_symmDiff.mp hsd with ⟨⟨⟨u, hu⟩, rfl, hv⟩, h'⟩ | ⟨⟨⟨u, hu⟩, rfl, hv⟩, h'⟩
+          · simp only [Form.image, Subtype.exists, exists_and_right, Set.mem_setOf_eq, not_exists,
+              not_and, forall_exists_index] at h'
+            have := Equiv.mem_union_symm_right <| Set.mem_union_right _ hw
+            conv at hw => rhs; exact Equiv.union_symm_apply_right this
+            have hu := Equiv.mem_union_symm_right hw
+            refine h' _ hu ?_ hv
+            symm; conv => lhs; exact Equiv.union_symm_apply_right this
+            exact Equiv.union_symm_apply_right hu
+          · simp only [Form.image, Subtype.exists, exists_and_right, Set.mem_setOf_eq, not_exists,
+              not_and, forall_exists_index] at h'
+            refine h' u (Or.inr (Or.inr hu)) ?_ hv
+            conv => lhs; exact Equiv.union_symm_apply_right <| Set.mem_union_right _ hu
+            exact Equiv.union_symm_apply_right hu
+        · refine iff_iff_eq.mpr <| hφ₂.2 _ _ ?_
+          refine Set.disjoint_left.mpr ?_; rintro x hsd rfl
+          rcases Set.mem_symmDiff.mp hsd with ⟨⟨⟨u, hu⟩, heq, hv⟩, h'⟩ | ⟨⟨⟨u, rfl⟩, heq, hv⟩, h'⟩
+          · simp only [Form.image, Subtype.exists, exists_and_right, Set.mem_setOf_eq, not_exists,
+              not_and, forall_exists_index] at h'
+            obtain rfl := Equiv.root_eq_par_symm heq.symm
+            exact h' _ (Set.mem_singleton _) rfl hv
+          · simp only [Form.image, Subtype.exists, exists_and_right, Set.mem_setOf_eq, not_exists,
+              not_and, forall_exists_index] at h'
+            refine h' _ (Set.mem_insert _ _) ?_ hv
+            conv => rhs; exact heq.symm
+            exact Equiv.union_symm_apply_left (Set.mem_singleton _)
+  · constructor
+    · intro ⟨hc, _⟩; contradiction
+    · rintro (rfl | ⟨hc, _⟩ | ⟨hc, _⟩) <;> exfalso <;> apply hz
+      · exact Set.mem_insert _ _
+      · right; left; exact hc
+      · right; right; exact hc
+
+lemma par_permute :
     (par_gen hx hx' hd hroot hφ₁ hφ₂).permute (Equiv.par e₁ e₂ hx hx' hd hy hy' hd') =
     par_gen (α := α.permute e₁) (β := β.permute e₂)
       hy hy' hd' hroot (par_form₁ hφ₁) (par_form₂ hφ₂) := by
   ext1
   · rfl
-  · sorry
-  · sorry
-  · sorry
+  · exact par_permute_rel _ _ _ _ _
+  · exact par_permute_lab _ _ _ _ _
+  · exact par_permute_form _ _ _ _ _
+
+end ParPermute
 
 lemma par_isomorphic {l : Type} [Bot l] {x y : Node} {ℓ : l} {α α' β β' : Lpo l}
     {hx : x ∉ α.nodes} {hx' : x ∉ β.nodes}
